Mt/Utils/List.lean
@@ -1,3 +1,5 @@
+import Mt.Utils.Fin
+
 namespace Mt.Utils.List
 
 theorem get_in {T : Type u} (l : List T) (idx : Fin l.length)
@@ -61,5 +63,31 @@ theorem eq_of_in_map {U V : Type u} {f : U -> V} {l : List U} {v : V}
       cases IH v_in_map_of_tail
       rename_i u u_hyp
       exact ⟨u, List.Mem.tail _ u_hyp.left, u_hyp.right⟩
+
+theorem get_congr {T : Type u} {l l' : List T} (idx : Fin l.length)
+  (eq : l = l')
+  : l.get idx = l'.get (Fin.cast idx (congrArg _ eq)) :=Eq.rec
+    (motive :=λ l' eq => l.get idx = l'.get (Fin.cast idx (congrArg _ eq)))
+    rfl eq
+
+theorem get_congr' {T : Type u} {l l' : List T}
+  {i : Fin l.length}
+  {j : Fin l'.length}
+  (l_eq : l = l')
+  (i_eq : i.val = j.val)
+  : l.get i = l'.get j :=by
+  have : j = Fin.cast i (congrArg _ l_eq) :=Fin.eq_of_val_eq i_eq.symm
+  rw [this]
+  exact get_congr _ l_eq
+
+theorem get_of_map {U V : Type u} {f : U -> V} {l : List U}
+  {idx : Fin (l.map f).length}
+  : (l.map f).get idx = f (l.get (Fin.cast idx (List.length_map l f))) :=
+  match l, idx with
+  | head :: tail, ⟨0, isLt⟩ => rfl
+  | head :: tail, ⟨n + 1, isLt⟩ => by
+    simp only [List.map, List.get]
+    rw [get_of_map]
+    rfl
 
 end Mt.Utils.List
